stdlib/Lean/Expr.lean
@@ -314,16 +314,16 @@ def Lean.Expr.symm : Expr → Expr
   | e  =>
     panic! s!"Expected an operator of Eq, Iff, SEq, HEq, Ne, Gt, Lt, Ge, Le, And, Or, but got {e.ctorName} :\n{e}"
 
-def Lean.Expr.decomposeType : Expr → Expr × Expr
+def Lean.Expr.decomposeComm : Expr → Expr × Expr
   | .app (.app (.app (.app (.const `letFun us) α) β) v) (.lam binderName binderType body binderInfo) =>
-    let args := body.decomposeType
+    let args := body.decomposeComm
     ⟨
       (Expr.const `letFun us).mkApp [α, β, v, .lam binderName binderType args.fst binderInfo],
       .letE binderName binderType v args.snd false
     ⟩
   | .letE declName type value body nondep =>
     let fn := fun body => .letE declName type value body nondep
-    body.decomposeType.map fn fn
+    body.decomposeComm.map fn fn
   | e  =>
     ⟨e.comm, e.symm⟩
 
